LeanSAT/AIG/LawfulOperator.lean
@@ -14,50 +14,57 @@ the AIGNET paper.
 
 namespace AIG
 
-abbrev UnaryOperator := (gate : Nat) → (aig : AIG) → (gate < aig.decls.size) → Entrypoint
+abbrev UnaryOperator :=
+    {α : Type} → [BEq α] → [Hashable α] → [DecidableEq α] →
+      (gate : Nat) → (aig : AIG α) → (gate < aig.decls.size) → Entrypoint α
 
 class LawfulUnaryOperator (f : UnaryOperator) where
-  le_size : ∀ (aig : AIG) (gate : Nat) (hgate), aig.decls.size ≤ (f gate aig hgate).aig.decls.size
-  decl_eq : ∀ (aig : AIG) (gate : Nat) (idx : Nat) (h1 : idx < aig.decls.size) (hgate) (h2),
-    (f gate aig hgate).aig.decls[idx]'h2 = aig.decls[idx]'h1
+  le_size {α : Type} [BEq α] [Hashable α] [DecidableEq α] : ∀ (aig : AIG α) (gate : Nat) (hgate),
+    aig.decls.size ≤ (f gate aig hgate).aig.decls.size
+  decl_eq {α : Type} [BEq α] [Hashable α] [DecidableEq α] : ∀ (aig : AIG α) (gate : Nat) (idx : Nat)
+      (h1 : idx < aig.decls.size) (hgate) (h2),
+        (f gate aig hgate).aig.decls[idx]'h2 = aig.decls[idx]'h1
 
 namespace LawfulUnaryOperator
 
 variable {f : UnaryOperator} [LawfulUnaryOperator f]
+variable {α : Type} [BEq α] [Hashable α] [DecidableEq α]
 
-theorem IsPrefix_aig (aig : AIG) (gate : Nat) {hgate} :
+theorem IsPrefix_aig (aig : AIG α) (gate : Nat) {hgate} :
     IsPrefix aig.decls (f gate aig hgate).aig.decls := by
   apply IsPrefix.of
   . intro idx h
     apply decl_eq
   . apply le_size
 
-theorem lt_mkNotCached_size (entry : Entrypoint) (gate : Nat) (hgate) :
+theorem lt_mkNotCached_size (entry : Entrypoint α) (gate : Nat) (hgate) :
     entry.start < (f gate entry.aig hgate).aig.decls.size := by
   have h1 := entry.inv
   have h2 : entry.aig.decls.size ≤ (f gate entry.aig hgate).aig.decls.size := by
     apply le_size
   omega
 
-theorem lt_size_of_lt_aig_size (aig : AIG) (gate : Nat) (hgate) (h : x < aig.decls.size)
+theorem lt_size_of_lt_aig_size (aig : AIG α) (gate : Nat) (hgate) (h : x < aig.decls.size)
     : x < (f gate aig hgate).aig.decls.size := by
-  have := le_size (f := f) aig gate hgate
-  omega
+  apply Nat.lt_of_lt_of_le
+  . exact h
+  . exact le_size aig gate hgate
 
-theorem le_size_of_le_aig_size (aig : AIG) (gate : Nat) (hgate) (h : x ≤ aig.decls.size)
+theorem le_size_of_le_aig_size (aig : AIG α) (gate : Nat) (hgate) (h : x ≤ aig.decls.size)
     : x ≤ (f gate aig hgate).aig.decls.size := by
-  have := le_size (f := f) aig gate hgate
-  omega
+  apply Nat.le_trans
+  . exact h
+  . exact le_size aig gate hgate
 
 @[simp]
-theorem denote_entry (entry : Entrypoint) {hgate} {h} :
+theorem denote_entry (entry : Entrypoint α) {hgate} {h} :
     ⟦(f gate entry.aig hgate).aig, ⟨entry.start, h⟩, assign ⟧
       =
     ⟦entry, assign⟧ :=  by
   apply denote.eq_of_aig_eq
   apply IsPrefix_aig
 
-theorem denote_mem_prefix {aig : AIG} {hgate} (h) :
+theorem denote_mem_prefix {aig : AIG α} {hgate} (h) :
     ⟦(f gate aig hgate).aig, ⟨start, by apply lt_size_of_lt_aig_size; omega⟩, assign⟧
       =
     ⟦aig, ⟨start, h⟩, assign⟧ :=  by
@@ -65,46 +72,52 @@ theorem denote_mem_prefix {aig : AIG} {hgate} (h) :
 
 end LawfulUnaryOperator
 
-abbrev BinaryOperator := (lhs rhs : Nat) → (aig : AIG) → (lhs < aig.decls.size) → (rhs < aig.decls.size) → Entrypoint
+abbrev BinaryOperator :=
+    {α : Type} → [BEq α] → [Hashable α] → [DecidableEq α] →
+      (lhs rhs : Nat) → (aig : AIG α) → (lhs < aig.decls.size) → (rhs < aig.decls.size) → Entrypoint α
 
 class LawfulBinaryOperator (f : BinaryOperator) where
-  le_size : ∀ (aig : AIG) (lhs rhs : Nat) (hl) (hr), aig.decls.size ≤ (f lhs rhs aig hl hr).aig.decls.size
-  decl_eq : ∀ (aig : AIG) (lhs rhs : Nat) (idx : Nat) (h1 : idx < aig.decls.size) (hl) (hr) (h2),
-    (f lhs rhs aig hl hr).aig.decls[idx]'h2 = aig.decls[idx]'h1
+  le_size {α : Type} [BEq α] [Hashable α] [DecidableEq α] : ∀ (aig : AIG α) (lhs rhs : Nat) (hl) (hr),
+    aig.decls.size ≤ (f lhs rhs aig hl hr).aig.decls.size
+  decl_eq {α : Type} [BEq α] [Hashable α] [DecidableEq α] : ∀ (aig : AIG α) (lhs rhs : Nat) (idx : Nat)
+    (h1 : idx < aig.decls.size) (hl) (hr) (h2),
+      (f lhs rhs aig hl hr).aig.decls[idx]'h2 = aig.decls[idx]'h1
 
 namespace LawfulBinaryOperator
 
 variable {f : BinaryOperator} [LawfulBinaryOperator f]
+variable {α : Type} [BEq α] [Hashable α] [DecidableEq α]
 
-theorem IsPrefix_aig (aig : AIG) (lhs rhs : Nat) {hl} {hr} :
+theorem IsPrefix_aig (aig : AIG α) (lhs rhs : Nat) {hl} {hr} :
     IsPrefix aig.decls (f lhs rhs aig hl hr).aig.decls := by
   apply IsPrefix.of
   . intro idx h
     apply decl_eq
   . apply le_size
 
-theorem lt_size (entry : Entrypoint) (lhs hrs : Nat) (hl) (hr)
+theorem lt_size (entry : Entrypoint α) (lhs hrs : Nat) (hl) (hr)
     : entry.start < (f lhs rhs entry.aig hl hr).aig.decls.size := by
   have h1 := entry.inv
   have h2 : entry.aig.decls.size ≤ (f lhs rhs entry.aig hl hr).aig.decls.size := by
     apply le_size
   omega
 
-theorem lt_size_of_lt_aig_size (aig : AIG) (lhs rhs : Nat) (hl hr)
+theorem lt_size_of_lt_aig_size (aig : AIG α) (lhs rhs : Nat) (hl hr)
     (h : x < aig.decls.size)
     : x < (f lhs rhs aig hl hr).aig.decls.size := by
-  have := le_size (f := f) aig lhs rhs hl hr
-  omega
+  apply Nat.lt_of_lt_of_le
+  . exact h
+  . exact le_size aig lhs rhs hl hr
 
 @[simp]
-theorem denote_entry (entry : Entrypoint) {hl} {hr} {h} :
+theorem denote_entry (entry : Entrypoint α) {hl} {hr} {h} :
     ⟦(f lhs rhs entry.aig hl hr).aig, ⟨entry.start, h⟩, assign ⟧
       =
     ⟦entry, assign⟧ :=  by
   apply denote.eq_of_aig_eq
   apply IsPrefix_aig
 
-theorem denote_mem_prefix {aig : AIG} {hl} {hr} (h) :
+theorem denote_mem_prefix {aig : AIG α} {hl} {hr} (h) :
     ⟦(f lhs rhs aig hl hr).aig, ⟨start, (by apply lt_size_of_lt_aig_size; omega)⟩, assign⟧
       =
     ⟦aig, ⟨start, h⟩, assign⟧ :=  by
